# UCMCO6602 - Cryptography and Encryption


I am a student in cryptography and would like to know more about the intuition behind combining modular math with logarithms - as a starting point to building creative solutions in cryptography. Please could you provide a simple/trivial example to illustrate encryption and decryption with the help of modular math and logarithms


Let me explain this with a simple example using discrete logarithms, which are fundamental to many cryptographic systems.

Let's consider a very basic (and not cryptographically secure) example to build intuition:

1. First, let's work in modulo 11 (a small prime number for simplicity)
2. Let's use 2 as our base (often called the generator)

In this system:
```python
# We work with the equation: 2^x mod 11
# Let's see what values we get:
2^1 mod 11 = 2
2^2 mod 11 = 4
2^3 mod 11 = 8
2^4 mod 11 = 5
2^5 mod 11 = 10
2^6 mod 11 = 9
2^7 mod 11 = 7
2^8 mod 11 = 3
2^9 mod 11 = 6
2^10 mod 11 = 1
```

The key insight is: given any result in this sequence, it's relatively easy to compute going forward (just multiply by 2 and take mod 11), but it's much harder to go backward (find x given 2^x mod 11) - this is called the discrete logarithm problem.

Here's a very simple encryption scheme based on this:
1. Say Alice wants to send message `m=3` to Bob
2. Bob chooses a secret key `k=4`
3. Bob's public key would be: `2^4 mod 11 = 5`
4. Alice encrypts by computing: `m * (public_key) mod 11 = 3 * 5 mod 11 = 4`
5. Bob decrypts using: `ciphertext * (2^(11-k)) mod 11 = 4 * (2^7) mod 11 = 4 * 7 mod 11 = 3`

Would you like me to elaborate on any part of this example or explain why this works mathematically?

This is a very simplified example for building intuition - real cryptographic systems use much larger numbers and more sophisticated techniques to ensure security. But the core idea of combining modular arithmetic with logarithms to create "easy forward, hard backward" operations remains central to many cryptographic protocols.



please could you show how to derive step 5 mathematically


Let me walk you through the mathematical derivation of step 5 (the decryption step).

Let's analyze it step by step:

1) In the encryption, we computed:
   ciphertext = m * (2^k mod 11) mod 11
   where m=3 and k=4

2) For decryption, we need to multiply by the inverse of (2^k mod 11)
   In modular arithmetic, for prime modulus p, we can use Fermat's Little Theorem:
   a^(p-1) ≡ 1 (mod p)

3) Therefore:
   2^10 ≡ 1 (mod 11)  [since 11-1 = 10]

4) This means:
   2^k * 2^(10-k) ≡ 1 (mod 11)
   
5) So, 2^(10-k) is the multiplicative inverse of 2^k in mod 11
   In our case, k=4, so we need 2^(10-4) = 2^6

6) Therefore, decryption works because:
   ```
   ciphertext * 2^(10-k) mod 11
   = [m * (2^k) * 2^(10-k)] mod 11
   = [m * 2^10] mod 11
   = [m * 1] mod 11  (since 2^10 ≡ 1 mod 11)
   = m mod 11
   ```

7) In our specific example:
   - Original message m = 3
   - Encrypted with k = 4 to get ciphertext = 4
   - Decrypt by computing: 4 * 2^6 mod 11
   - 2^6 mod 11 = 9
   - 4 * 9 mod 11 = 36 mod 11 = 3
   - We get back our original message m = 3

This demonstrates how modular arithmetic provides a way to undo the encryption by using properties like Fermat's Little Theorem to find multiplicative inverses. The security relies on the difficulty of finding k given 2^k mod 11 (the discrete logarithm problem), even though the math of encryption/decryption is straightforward if you know k.

Would you like me to elaborate on any of these steps or explain more about how Fermat's Little Theorem works in this context?

please can you explain step 2 relating to fermats little theorem - in more detail

Let me explain Fermat's Little Theorem and its significance in our cryptographic context in detail.

Fermat's Little Theorem states: 
For any integer a and prime number p, if p doesn't divide a, then:
a^(p-1) ≡ 1 (mod p)

Let's understand this in several ways:

1) First, let's verify it for our case (a=2, p=11) by listing out powers of 2 mod 11:
```python
2^1 mod 11 = 2
2^2 mod 11 = 4
2^3 mod 11 = 8
2^4 mod 11 = 5
2^5 mod 11 = 10
2^6 mod 11 = 9
2^7 mod 11 = 7
2^8 mod 11 = 3
2^9 mod 11 = 6
2^10 mod 11 = 1  # This is p-1 = 11-1 = 10th power
```

2) We can understand why this works by considering the sequence of remainders when dividing powers of a by p:
   - If p is prime and a is not divisible by p
   - Then multiplying by a each time must give different remainders (until we cycle)
   - There are only p-1 possible non-zero remainders (1 to p-1)
   - Therefore, after at most p-1 steps, we must get back to where we started
   - The first remainder must be the same as remainder after p-1 steps
   - This means a^(p-1) ≡ 1 (mod p)

3) In our cryptographic application, this theorem is crucial because:
   - We need to find the multiplicative inverse of 2^k mod 11
   - The theorem tells us that 2^10 ≡ 1 (mod 11)
   - Therefore: 2^k * 2^(10-k) ≡ 1 (mod 11)
   - This means 2^(10-k) is the multiplicative inverse we need!

4) Let's verify this with k=4:
   - We need the inverse of 2^4 mod 11 = 5
   - The theorem tells us to use 2^(10-4) = 2^6 = 9 mod 11
   - Check: 5 * 9 = 45 ≡ 1 (mod 11) ✓

This is why in our decryption step:
```
ciphertext * 2^(10-k) mod 11
= [m * (2^k) * 2^(10-k)] mod 11
= m * (2^k * 2^(10-k)) mod 11
= m * 1 mod 11  [because 2^k * 2^(10-k) ≡ 1 (mod 11)]
= m
```

The beauty of Fermat's Little Theorem in cryptography is that it guarantees we can always find multiplicative inverses modulo a prime number, which is essential for decryption. This property of prime numbers (and the fact that the discrete logarithm problem is hard) is what makes many cryptographic systems possible.

Would you like me to:
1) Prove Fermat's Little Theorem more rigorously?
2) Show more examples with different values?
3) Explain how this extends to more practical cryptographic systems?

is (a*b) mod c , the same as (a mod c) *( b mod c)

Let me help you understand this important property of modular arithmetic!

Yes, (a*b) mod c is equivalent to ((a mod c) * (b mod c)) mod c

This is known as the property of modular multiplication or the "multiplication rule for congruences." Let me demonstrate why this is true and provide some examples:

1) Mathematical Proof:
   Let's say: 
   a = mc + r₁  (where r₁ is remainder when a÷c)
   b = nc + r₂  (where r₂ is remainder when b÷c)

   Then:
   a*b = (mc + r₁)(nc + r₂)
       = mnc² + mr₂c + nr₁c + r₁r₂
       = c(mnc + mr₂ + nr₁) + r₁r₂

   Therefore:
   (a*b) mod c = (r₁r₂) mod c
   
   And since r₁ = a mod c and r₂ = b mod c,
   This shows: (a*b) mod c = ((a mod c) * (b mod c)) mod c

2) Let's verify with some examples:

```python
# Example 1:
a = 17, b = 15, c = 7

(17 * 15) mod 7
= 255 mod 7
= 3

(17 mod 7) * (15 mod 7) mod 7
= 3 * 1 mod 7
= 3

# Example 2:
a = 25, b = 12, c = 6

(25 * 12) mod 6
= 300 mod 6
= 0

(25 mod 6) * (12 mod 6) mod 6
= 1 * 0 mod 6
= 0
```

3) Why this is important:
   - This property allows us to reduce intermediate results in calculations, preventing numbers from getting too large
   - In cryptography, this is crucial because we often work with very large numbers
   - Instead of multiplying large numbers and then taking modulo, we can:
     * First reduce the numbers by taking their modulo
     * Then multiply the smaller numbers
     * Take modulo of the result

4) Practical example in cryptography:
```python
# When computing something like:
(2^1000 mod 11)

# Instead of computing 2^1000 (huge number) then taking mod 11
# We can compute step by step:
2^1 mod 11 = 2
(2 * 2) mod 11 = 4
(4 * 2) mod 11 = 8
...and so on
```

This property is particularly useful in:
- Implementing efficient modular exponentiation
- RSA encryption/decryption
- Digital signatures
- Any cryptographic protocol involving large number arithmetic

Would you like me to elaborate on any of these aspects or show how this property is used in a specific cryptographic application?

please could you define this relationship in simple terms:  a^(p-1) ≡ 1 (mod p) . Then pleae could you show using a simple brute force worked example that this relationship holds.

Let me break this down:

1) Simple Definition of a^(p-1) ≡ 1 (mod p):
   - When we raise any number 'a' to the power of (p-1)
   - And then divide by prime number p
   - The remainder will be 1
   - (As long as 'a' is not divisible by p)

2) Let's verify this with a simple example:
   Let's use p = 7 (prime) and a = 2

   Let's compute all powers of 2 modulo 7:
   ```python
   2^1 mod 7 = 2
   2^2 mod 7 = 4
   2^3 mod 7 = 1
   2^4 mod 7 = 2
   2^5 mod 7 = 4
   2^6 mod 7 = 1  # This is 2^(p-1) since p=7
   ```

   Let's verify step by step for 2^6:
   ```
   2^6 = 2 × 2 × 2 × 2 × 2 × 2
   = 64
   
   64 ÷ 7 = 9 remainder 1
   
   Therefore: 2^6 ≡ 1 (mod 7)
   ```

3) Let's try another example:
   Let's use p = 5 (prime) and a = 3

   ```python
   3^1 mod 5 = 3
   3^2 mod 5 = 4
   3^3 mod 5 = 2
   3^4 mod 5 = 1  # This is 3^(p-1) since p=5
   ```

   Let's verify 3^4:
   ```
   3^4 = 3 × 3 × 3 × 3
   = 81
   
   81 ÷ 5 = 16 remainder 1
   
   Therefore: 3^4 ≡ 1 (mod 5)
   ```

This relationship is powerful because:
- It works for ANY number 'a' not divisible by p
- It works for ANY prime p
- The result is ALWAYS 1

Would you like me to:
1) Try more examples with different values?
2) Show how this is used practically in cryptography?
3) Explain why this property is so important for finding multiplicative inverses?

